theories/lib/assert.v
@@ -11,7 +11,7 @@ Notation "'assert:' e" := (assert (λ: <>, e))%E (at level 99) : expr_scope.
 Lemma rel_assert_l `{!relocG Σ} K e t A :
   (∀ K t A, (REL fill K (of_val #true) << t : A) -∗ REL fill K e << t : A) -∗
   (▷ REL fill K (of_val #()) << t : A) -∗
-  REL fill K (assert (LamV BAnon e)%V) << t : A.
+  REL fill K (assert: e)%V << t : A.
 Proof.
   iIntros "H1 H2". rel_rec_l. rel_rec_l.
   rel_apply_l "H1". by rel_if_l.
